\documentclass[]{article}
\usepackage{graphicx,amsmath,amsthm, amssymb,setspace}
\usepackage[a4paper, total={6in, 8.5in}]{geometry}
\newcommand\ddfrac[2]{\frac{\displaystyle #1}{\displaystyle #2}}
%opening
\title{}
\author{}

\begin{document}

\maketitle

\begin{abstract}

\end{abstract}

\section{}


For $\alpha>0$, $k\geq 1$, define 
\[I(\alpha,k) = \int_{\alpha}^\infty x^{k/2} e^{-x/2} dx. \]
Note that $I(\alpha,0)=2e^{-\alpha/2}$. Furthermore, it can be shown by integration by parts that, for $k\geq 0$,
\begin{align}\label{iterative}
I(\alpha,k) =  2\alpha^{k/2} e^{-\alpha/2}+kI(\alpha,k-2).
\end{align}
Let $Z\sim \chi^2(k)$, $k\geq 2$. The density of $Z$ is
\[ f(x) = \frac{1}{2^{k/2}\Gamma(k/2)} x^{k/2-1}e^{-x/2}.  \]
For $\alpha>0$, $k\geq 2$, by \eqref{iterative},
\begin{align*}
E(Z\mid Z>\alpha)&= \ddfrac{\int_{\alpha}^\infty xf(x) dx}{\int_{\alpha}^\infty f(x) dx} = \dfrac{I(\alpha,k)}{I(\alpha,k-2)} \\[1ex]
& =  \dfrac{2\alpha^{k/2} e^{-\alpha/2}}{I(\alpha,k-2)}+k\\
&= \ddfrac{2\alpha^{k/2} e^{-\alpha/2}}{2\alpha^{k/2-1} e^{-\alpha/2}+kI(\alpha, k-4)}+k \\[1ex]
&< \alpha+k.
\end{align*}
For $k=1$, the above inequality needs to be modified slightly.
It is clear that $E(Z|Z>\alpha)>\alpha$. 
When $\alpha$ is large, $k>0$ is constant and $\alpha>>k$, by \eqref{iterative}, (not sure for the part below)
\begin{align}\label{big_Theta}
I(\alpha,k) = \Theta(2\alpha^{k/2}e^{\alpha/2}).
\end{align}
Hence (not sure for the part below)
\begin{align*}
E(Z|Z>\alpha)&=\ddfrac{2\alpha^{k/2} e^{-\alpha/2}}{2\alpha^{k/2-1} e^{-\alpha/2}+k\Theta(2\alpha^{k/2-2}e^{\alpha/2})}+k \\[1ex]
&=\dfrac{\alpha}{1+2k\Theta(\alpha^{-2})}+k.
\end{align*}
\end{document}
